working on Jones & Duponcheel stuff

jed_JD.v
@@ -21,8 +21,10 @@ Unset Transparent Obligations.
 (* 
 Set Printing Coercions.
 Set Printing Implicit.
+Set Printing Notations.
 Unset Printing Coercions.
 Unset Printing Implicit.
+Unset Printing Notations.
 *)
 
 Section CMN. (* category C and monads M and N *)
@@ -30,22 +32,36 @@ Section CMN. (* category C and monads M and N *)
 Context {C : Category}.
 Context {M : obj[C] -> obj[C]}.
 Context {N : obj[C] -> obj[C]}.
-Context {M3 : @Monad3 C M}.
-Context {N3 : @Monad3 C N}.
+Context (M3 : @Monad3 C M).
+Context (N3 : @Monad3 C N).
 
 Print Implicit join3.
 Print Implicit map3.
 Print Implicit ret3.
 Print Implicit ext.
 
-(* uses given definition for join of MN, expressed using ext *)
+(* this is the prod construction conditions of Jones & Duponcheel,
+  expressed using their definitions of unitMN and mapMN and joinMN ;
+  for joinMN we write it using ext *)
+
+Definition retc x := @ret3 C M M3 _ ∘ @ret3 C N N3 x.
+Definition mapc {x y} f := map3 M3 (@map3 C N N3 x y f).
+
 Record JD_P : Type := 
   { prod : ∀ x : obj[C], N (M (N x)) ~{ C }~> M (N x) ;
     P1 : ∀ x y (f : x ~{ C }~> y), 
-      prod y ∘ map3 N3 (map3 M3 (map3 N3 f)) ≈ map3 M3 (map3 N3 f) ∘ prod x ;
+      prod y ∘ map3 N3 (mapc f) ≈ mapc f ∘ prod x ;
     P2 : ∀ x, prod x ∘ ret3 N3 ≈ id ;
-    P3 : ∀ x, prod x ∘ map3 N3 (ret3 M3 ∘ ret3 N3) ≈ ret3 M3 ;
+    P3 : ∀ x, prod x ∘ map3 N3 (retc x) ≈ ret3 M3 ;
     P4 : ∀ x, prod x ∘ map3 N3 (ext M3 (prod x)) ≈ ext M3 (prod x) ∘ prod _ }.
+
+Definition join_P (P : JD_P) x := ext M3 (prod P x).
+Definition pext_P (P : JD_P) {x y} (f : x ~> M (N y)) := prod P y ∘ map3 N3 f.
+
+Lemma pext_P_respects (P : JD_P) (x y : obj[C]) :
+  Proper (equiv ==> equiv) (@pext_P P x y).
+Proof. proper. unfold pext_P.  apply comp_o_l.
+apply map3_respects. apply X. Qed.
 
 Print Implicit JD_P.
 Print Implicit P4.
@@ -54,28 +70,70 @@ Print Implicit m_assoc.
 Print Implicit m_id_l.
 Print Implicit m_id_r.
 
+Record JD_Pext : Type := 
+  { pext : ∀ {x y : obj[C]} (f : x ~{ C }~> M (N y)), N x ~{ C }~> M (N y) ;
+    pext_respects : ∀ x y : obj[C], Proper (equiv ==> equiv) (@pext x y) ;
+    pext_o : ∀ x y z (f : x ~{ C }~> y) (g : y ~> M (N z)), 
+      pext (g ∘ f) ≈ pext g ∘ map3 N3 f ;
+    Pext1 : ∀ x y (f : x ~{ C }~> y), pext (mapc f) ≈ mapc f ∘ pext id ;
+    Pext2 : ∀ x y (f : x ~{ C }~> M (N y)), pext f ∘ ret3 N3 ≈ f ;
+    Pext3 : ∀ x, pext (retc x) ≈ ret3 M3 ;
+    Pext4 : ∀ x y f, pext (ext M3 (@pext x y f)) ≈ ext M3 (pext f) ∘ pext id }.
+
+Program Definition JD_P_Pext (P : JD_P) : JD_Pext :=
+  {| pext := fun x y f => prod P y ∘ map3 N3 f |}.
+Next Obligation. proper. unfold pext_P.  apply comp_o_l.
+apply map3_respects. apply X. Qed.
+Next Obligation. rewrite map3_comp. apply comp_assoc. Qed.
+Next Obligation. rewrite map3_id, id_right. apply P1. Qed.
+Next Obligation. rewrite <- comp_assoc. unfold map3.
+rewrite m_id_r. rewrite comp_assoc. rewrite P2. apply id_left. Qed.
+Next Obligation. apply P3. Qed.
+Next Obligation. pose (map3_respects N3). rewrite ext_o.
+rewrite map3_comp. rewrite comp_assoc. rewrite P4.
+rewrite map3_id, id_right. rewrite <- !comp_assoc.
+apply comp_o_l. apply P1. Qed.
+
 Check jed_monad.Monad_from_3_obligation_1.
 Check jed_monad.Monad_from_3_obligation_2.
 Check jed_monad.Monad_from_3_obligation_3.
 
 Check jed_monad.Functor_from_3_obligation_3.
+Check JD_P_Pext_obligation_6.
 
 (* P1 to P4 give monad in Kleisli category of M *)
 Program Definition JD_P_NK (P : JD_P) : @Monad3 (@Kleisli_from_3 C M M3) N :=
   {| ret3 := fun x : obj[C] => ret3 M3 ∘ @ret3 _ _ N3 x ;
-    ext := fun (x y : obj[C]) (f : x ~> M (N y)) => prod P y ∘ map3 N3 f |}.
-
-Next Obligation. proper. pose (map3_respects N3).  rewrite X. reflexivity. Qed.
-
-Next Obligation. rewrite comp_assoc.  rewrite m_id_r.  rewrite <- comp_assoc.
+    ext := fun (x y : obj[C]) (f : x ~> M (N y)) => pext_P P f |}.
+Next Obligation. proper. apply pext_P_respects.  rewrite X. reflexivity. Qed.
+Next Obligation. rewrite comp_assoc.  rewrite m_id_r.
+unfold pext_P. rewrite <- comp_assoc.
 rewrite <- (jed_monad.Monad_from_3_obligation_1 N3).
 rewrite comp_assoc.  rewrite P2.  apply id_left. Qed.
-
 Next Obligation. apply P3. Qed.
-Next Obligation.  pose (map3_respects N3).  rewrite !ext_o.
-rewrite !jed_monad.Functor_from_3_obligation_3.
-rewrite !comp_assoc.  rewrite P4.  apply comp_o_r.
+Next Obligation.  pose (map3_respects N3).  unfold pext_P. rewrite !ext_o.
+rewrite !map3_comp.  rewrite !comp_assoc.  rewrite P4.  apply comp_o_r.
 rewrite <- !comp_assoc.  apply comp_o_l.  symmetry.  apply P1. Qed.
+
+Check JD_P_NK_obligation_1.
+Check JD_P_NK_obligation_2.
+Check JD_P_NK_obligation_3.
+Check JD_P_NK_obligation_4.
+
+Program Definition JD_Pext_NK (P : JD_Pext) :
+  @Monad3 (@Kleisli_from_3 C M M3) N := {| ret3 := retc ;
+    ext := fun (x y : obj[C]) (f : x ~> M (N y)) => pext P f |}.
+Next Obligation. apply pext_respects. Qed.
+Next Obligation. unfold retc. rewrite comp_assoc, m_id_r. apply Pext2. Qed.
+Next Obligation. apply Pext3. Qed.
+Next Obligation. rewrite pext_o. rewrite Pext4.
+rewrite <- comp_assoc. rewrite <- pext_o. 
+pose pext_respects.  rewrite id_left. reflexivity. Qed.
+
+Check JD_Pext_NK_obligation_1.
+Check JD_Pext_NK_obligation_2.
+Check JD_Pext_NK_obligation_3.
+Check JD_Pext_NK_obligation_4.
 
 Print Implicit fmap.
 Print Implicit ret3.
@@ -85,3 +143,71 @@ Print Implicit join3.
 Print Implicit map3.
 
 End CMN. (* more to be done, but this lets the file compile *)
+
+(* compound monad, monad in Kleisli category of another monad *)
+(* this is the basis of the prod construction of Jones & Duponcheel *)
+
+Program Definition MinK_comp {C M} (H : @Monad3 C M) {N} 
+  (J : @Monad3 (@Kleisli_from_3 C M H) N) : @Monad3 C (Basics.compose M N) :=
+  {| ret3 := @ret3 _ _ J ; ext := fun x y f => ext H (ext J f) |}.
+
+Next Obligation.  proper. apply ext_respects.
+apply (ext_respects J). apply X. Qed.
+
+Next Obligation.  (* rewrite (m_id_r J). or rewrite m_id_r. fail here *)
+exact (m_id_r J _ _ f). Qed.
+
+Next Obligation. pose (ext_respects H). (* needed, including the H *)
+rewrite m_id_l. apply m_id_l. Qed.
+
+Next Obligation. rewrite m_assoc. apply ext_respects.
+(* apply setoid_trans. fails, why?? and rewrite (m_assoc J). fails *)
+apply (m_assoc J _ _ _ g f). Qed.
+
+Check MinK_comp.
+
+Print Implicit join3.
+
+(* when we have a compound monad defined in this way, it satisfies J(1) *)
+Lemma MinK_J1 {C M} (H : @Monad3 C M) {N} 
+  (J : @Monad3 (@Kleisli_from_3 C M H) N) x : 
+  ext H (join3 (MinK_comp H J)) ≈ @join3 _ _ (MinK_comp H J) x ∘ join3 H.
+Proof. simpl. apply ext_ext. Qed.
+
+(* monad in Kleisli category of another monad, implies Pext rules *)
+(* or does it?? maybe it requires the J1 condition
+Program Definition MinK_Pext {C M} (M3 : @Monad3 C M) {N} (N3 : @Monad3 C N)
+  (J : @Monad3 (@Kleisli_from_3 C M M3) N) : JD_Pext M3 N3 :=
+  {| pext := fun x y (f : x ~> M (N y)) => ext J f |}.
+Next Obligation.  proper.  apply (ext_respects J). apply X. Qed.
+Next Obligation.  rewrite !m_id_r. what to do now
+
+Program Definition MinK_P {C M} (M3 : @Monad3 C M) {N} (N3 : @Monad3 C N)
+  (J : @Monad3 (@Kleisli_from_3 C M M3) N) : JD_P M3 N3 :=
+  {| prod := fun x => ext J (@id C (M (N x))) |}.
+*)
+
+Print Implicit ext_respects.
+Print Implicit Kleisli_from_3.
+Print Implicit Monad3.
+Print Implicit m_assoc.
+Print Implicit k_adj.
+Print Implicit Adjunction_IffEq_comp.
+Print Monad3.
+Print Implicit AIE_to_Monad3.
+Check AIE_to_Monad3.
+
+(* we can prove MinK_comp using Adjunction_IffEq_comp, as
+  both monads give rise to adjunctions (using Kleisli categories),
+  compose these adjunctions, get compound monad from that,
+  however this obscures us seeing the construction *)
+Lemma MinK_comp_adj {C M} (H : @Monad3 C M) {N} 
+  (J : @Monad3 (@Kleisli_from_3 C M H) N) : @Monad3 C (Basics.compose M N).
+Proof.  pose (Adjunction_IffEq_comp (k_adj J) (k_adj H)).
+exact (AIE_to_Monad3 a). Defined.
+Check MinK_comp_adj.
+
+(* this shows the type of ext, not how it is defined *)
+Check (fun H J => ext (MinK_comp_adj H J)). 
+Check (fun H J => ext (MinK_comp H J)). 
+
